%!TEX root = ./main.tex
%!TEX encoding = UTF-8 Unicode

\section{The Variation Principle and the Noether Theorem}

We return to a single-particle system. The Heisenberg equation of motion, describing the time evolution of a particle at position $\hat{\bm r}$ having momentum $\hat{\bm p}$, is given by
\be
\ii\hbar\frac{\dd}{\dd t}\hat{\bm r}(t)=[\hat{\bm r}(t),\hat H]=\left.\ii\hbar\frac{\partial H(\bm r,\bm p)}{\partial\bm p}\right|_{\substack{\bm r=\hat{\bm r}(t)\\ \bm p=\hat{\bm p}(t)}},
\ee\be
\ii\hbar\frac{\dd}{\dd t}\hat{\bm p}(t)=-[\hat{\bm r}(t),\hat H]=\left.\ii\hbar\frac{\partial H(\bm r,\bm p)}{\partial\bm r}\right|_{\substack{\bm r=\hat{\bm r}(t)\\ \bm p=\hat{\bm p}(t)}}.
\ee